gol_in_gol_circuitScript.sml
@@ -6,10 +6,42 @@ open gol_simLib gol_rulesTheory boolSyntax computeLib cv_transLib
 
 val _ = new_theory "gol_in_gol_circuit";
 
+Definition union_blist2_def:
+  union_blist2 _ NONE Nil ls = ls ∧
+  union_blist2 m NONE (Falses n ls1) ls = union_blist2 (m + n) NONE ls1 ls ∧
+  union_blist2 m NONE (Cell a ls1) ls = union_blist2 m (SOME a) ls1 ls ∧
+  union_blist2 m (SOME a) ls1 Nil = Nil ∧
+  union_blist2 m (SOME a) ls1 (Falses n ls) = (
+    if m < n then mk_Falses m (Cell a (union_blist2 0 NONE ls1 (Falses (n - (m + 1)) ls)))
+    else mk_Falses n (union_blist2 (m - n) (SOME a) ls1 ls)) ∧
+  union_blist2 m (SOME a) ls1 (Cell b ls) = (
+    if m = 0 then Cell (build_Or a b) (union_blist2 0 NONE ls1 ls)
+    else Cell b (union_blist2 (m - 1) (SOME a) ls1 ls))
+End
+
+Theorem union_blist_eq:
+  (∀m ls1 ls. union_blist m ls1 ls = union_blist2 m NONE ls1 ls) ∧
+  (∀m a ls1 ls. union_blist' m a ls1 ls = union_blist2 m (SOME a) ls1 ls)
+Proof
+  HO_MATCH_MP_TAC union_blist_ind
+  \\ simp [union_blist_def, union_blist2_def]
+QED
+
+(* val _ = cv_transLib.cv_trans_rec union_blist2_def (
+  WF_REL_TAC ‘measure (λ_,_,ls1,ls. cv$cv_size ls1 + cv$cv_size ls)’
+  \\ Cases \\ gvs [] \\ rw [] \\ gvs [])
+  (fn goal => (set_goal goal; PolyML.print goal; NO_TAC goal))
+) *)
+
+val _ = cv_transLib.cv_trans_rec union_blist2_def cheat
+val _ = cv_transLib.cv_trans union_blist_eq
+val _ = cv_transLib.cv_auto_trans build_mega_cell_def
+
 Theorem floodfill_result = floodfill diag params;
 
-val _ = cv_transLib.cv_auto_trans test_pt_slow_def
-val _ = cv_transLib.cv_auto_trans $ definition "main_circuit_def"
+val _ = cv_transLib.cv_auto_trans test_blists_def
+val _ = cv_transLib.cv_trans_deep_embedding EVAL $
+  definition "main_circuit_def"
 
 Definition build_mega_cells_def:
   build_mega_cells = mega_cell_builder main_circuit
@@ -19,7 +51,7 @@ Theorem gol_in_gol_thm:
   gol_in_gol build_mega_cells (^periodN * 60) read_mega_cells
 Proof
   rewrite_tac [build_mega_cells_def]
-  \\ irule floodfill_finish \\ simp [floodfill_result]
+  \\ irule floodfill_result_finish \\ simp [floodfill_result]
   \\ CONV_TAC cv_eval
 QED
 
@@ -33,4 +65,5 @@ Proof
   \\ metis_tac [arithmeticTheory.MULT_ASSOC]
 QED
 
+val _ = (max_print_depth := 10); (* avoids blow up in size of Theory.sig file *)
 val _ = export_theory();
